typeExtractionSem.v: reduce reliance on closedness

theories/DSub/typeExtractionSem.v
@@ -28,41 +28,62 @@ Section interp_equiv.
   Qed.
 
   (** However, a stamp semantics that carries over to saved predicates must use
-      σ in ρ. And the result is only equivalent for closed ρ with the expected length. *)
-  Definition interp_extractedTy: (ty * vls) → envD Σ :=
-    λ '(T, σ) ρ v, (⟦ T ⟧ (to_subst σ >> ρ) v)%I.
-  Notation "⟦ T ⟧ [ σ ]" := (interp_extractedTy (T, σ)).
-
-  Definition envD_equiv n φ1 φ2: iProp Σ :=
-    (∀ ρ v, φ1 (to_subst ρ) v ≡ φ2 (to_subst ρ) v)%I.
-  Notation "φ1 ≈[  n  ] φ2" := (envD_equiv n φ1 φ2) (at level 70).
+      σ in ρ. *)
+  Definition interp_extractedTy: ty → env → envD Σ :=
+    λ T σ ρ, ⟦ T ⟧ (σ >> ρ).
+  Notation "⟦ T ⟧ [ σ ]" := (interp_extractedTy T σ).
+  Global Arguments interp_extractedTy /.
 
   Lemma extraction_envD_equiv g s σ T n:
     T ~[ n ] (g, (s, σ)) →
-    (∃ T', ⌜ g !! s = Some T'⌝ ∧
-        ⟦ T ⟧ ≈[ n ] ⟦ T' ⟧ [ σ ])%I.
+    ∃ T', g !! s = Some T' ∧ ⟦ T ⟧ ≡ ⟦ T' ⟧ [ to_subst σ ].
   Proof.
-    iIntros ((T' & -> & <- & _ & _)). iExists _; iSplit => //.
-    iIntros (ρ v) "!%".
-    rewrite /interp_extractedTy. exact: interp_subst_compose.
+    intros (T' & -> & <- & _ & _). eexists _; split => //.
+    intros ρ v. exact: interp_subst_compose.
   Qed.
 
-  (** envD_equiv commutes with substitution. *)
+  (** [envD_equiv] commutes with infinite substitution. *)
+  Lemma envD_equiv_infsubst {g T m n ξ s1 σ1 s2 σ2}:
+    T ~[ m ] (g, (s1, σ1)) →
+    T.|[ξ] ~[ n ] (g, (s2, σ2)) →
+    ∃ T1 T2, g !! s1 = Some T1 ∧ g !! s2 = Some T2 ∧
+    ⟦ T1 ⟧ [ to_subst σ1 >> ξ ] ≡ ⟦ T2 ⟧ [ to_subst σ2 ].
+  Proof.
+    intros (T1 & -> & <- & _ & _) (T2 & -> & Heq2 & _ & _).
+    exists T1, T2; split_and! => // ρ v /=.
+    rewrite (interp_subst_ids T1 _ _) (interp_subst_ids T2 _ _). f_equiv.
+    move: Heq2 => /(f_equal (λ T, T.|[ρ])). by asimpl.
+  Qed.
+
+  (** [envD_equiv] commutes with finite substitution, but under extra
+      assumptions on the substitutions in questions (on free variables and
+      length). *)
   Lemma envD_equiv_subst g T m n ξ s1 σ1 s2 σ2:
     T ~[ m ] (g, (s1, σ1)) →
     T.|[to_subst ξ] ~[ n ] (g, (s2, σ2)) →
     length ξ = m →
     nclosed_σ ξ n →
-    (∃ T1 T2, ⌜ g !! s1 = Some T1⌝ ∧ ⌜ g !! s2 = Some T2 ⌝ ∧
-    ⟦ T1 ⟧ [ σ1.|[to_subst ξ] ] ≈[ n ] ⟦ T2 ⟧ [ σ2 ])%I.
+    ∃ T1 T2, g !! s1 = Some T1 ∧ g !! s2 = Some T2 ∧
+    ⟦ T1 ⟧ [ to_subst σ1.|[to_subst ξ] ] ≡ ⟦ T2 ⟧ [ to_subst σ2 ].
   Proof.
-    rewrite /interp_extractedTy; iIntros ((T1 & -> & Heq1 & Hclσ1 & HclT1) (T2 & -> & Heq2 & Hclσ2 & HclT2) Hlenξ Hclξ).
-    iExists _, _; repeat iSplit => //; iIntros (ρ v) "/= !%".
-    have Hrew: T2.|[to_subst σ2].|[to_subst ρ] =
-      T1.|[to_subst σ1.|[to_subst ξ]].|[ to_subst ρ].
-    by erewrite !subst_compose, Heq2, Heq1.
-    asimpl in Hrew.
-    rewrite (interp_subst_ids T1 _ _) (interp_subst_ids T2 _ _) Hrew //.
+    intros (T1 & -> & <- & Hclσ1 & HclT1) (T2 & -> & Heq2 & Hclσ2 & HclT2) Hlenξ Hclξ.
+    exists T1, T2; split_and! => // ρ v /=.
+    rewrite (interp_subst_ids T1 _ _) (interp_subst_ids T2 _ _). f_equiv.
+    have: T1.|[to_subst σ1.|[to_subst ξ]] = T2.|[to_subst σ2].
+    - by rewrite Heq2 (subst_compose HclT1 _ Hclσ1 _ Hclξ).
+    - move => /(f_equal (λ T, T.|[ρ])). by asimpl.
+    (* Reusing envD_equiv_infsubst takes more work than proving it from scratch! *)
+    (* Restart.
+    intros Hext1 Hext2 Hlen Hclξ.
+    destruct (envD_equiv_infsubst Hext1 Hext2) as (T1 & T2 & Hgs1 & Hgs2 & Heq).
+    destruct Hext1 as (T1' & Hgs1' & Heq1 & Hclσ1 & HclT1).
+    have ?: T1' = T1 by simplify_eq. subst. simplify_eq.
+    exists T1, T2; split_and! => // ρ v /=.
+    move: (Heq ρ v) => /= <- {Heq}.
+    have: T1.|[to_subst σ1.|[to_subst ξ]] = T1.|[to_subst σ1 >> to_subst ξ].
+    - rewrite (subst_compose HclT1 _ Hclσ1 _ Hclξ) //. by asimpl.
+    - move => /(f_equal (λ T, T.|[ρ])). asimpl.
+      rewrite !(interp_subst_ids T1 _ _). by move->. *)
   Qed.
 
   Lemma alloc_sp T: (|==> ∃ γ, γ ⤇ ty_interp T)%I.
